AwsCryptographicMaterialProviders/dafny/AwsCryptographyKeyStore/test/TestCreateKeys.dfy
@@ -37,7 +37,10 @@ module TestCreateKeys {
 
     var keyStore :- expect KeyStore.KeyStore(keyStoreConfig);
 
-    var branchKeyId :- expect keyStore.CreateKey(Types.CreateKeyInput());
+    var branchKeyId :- expect keyStore.CreateKey(Types.CreateKeyInput(
+      branchKeyIdentifier := None,
+      encryptionContext := None
+    ));
 
     var beaconKeyResult :- expect keyStore.GetBeaconKey(
       Types.GetBeaconKeyInput(
@@ -78,7 +81,8 @@ module TestCreateKeys {
       branchKeyIdActiveVersion,
       "",
       "",
-      keyArn
+      keyArn,
+      map[]
     );
 
     var output := DDBKeystoreOperations.WriteNewKeyToStore(
@@ -101,7 +105,8 @@ module TestCreateKeys {
       "!= branchKeyIdActiveVersion",
       "",
       "",
-      keyArn
+      keyArn,
+      map[]
     );
 
     var output := DDBKeystoreOperations.WriteNewKeyToStore(
